Finish proof that elim_let preserves alpha
Finished proof of substitution result
Not easy to prove same_in_t, doesnt hold in general
Instead, prove notin bnd implies this
Change def of elim_let to alpha convert always
Finish all proofs for elim_let alpha

proofs/transform/eliminate_let.v
@@ -8,11 +8,164 @@ Set Bullet Behavior "Strict Subproofs".
 (*First version (not why3's)*)
 Section ElimLetAlt.
 
+(*Alternate [safe_sub_t] that always alpha converts.
+  Nicer for proofs.
+  Comments in [ElimLet.v] describe why we need this*)
+Definition safe_sub_t' (t1: term) (x: vsymbol) (t2: term) : term :=
+  if aset_mem_dec x (tm_fv t2)
+  then sub_t t1 x (a_convert_t t2 (aset_union (tm_fv t1) (tm_fv t2))) else t2.
+
+Definition safe_sub_f' (t1: term) (x: vsymbol) (f2: formula) : formula :=
+  if aset_mem_dec x (fmla_fv f2)
+  then sub_f t1 x (a_convert_f f2 (aset_union (tm_fv t1) (fmla_fv f2))) else f2.
+
+(*TODO: move all this to Alpha.v*)
+Lemma safe_sub_t_typed' {gamma} (t1 : term) (x : string) (t2 : term) (ty1 ty2 : vty):
+  term_has_type gamma t1 ty1 ->
+  term_has_type gamma t2 ty2 -> 
+  term_has_type gamma (safe_sub_t' t1 (x, ty1) t2) ty2.
+Proof.
+  intros Hty1 Hty2.
+  unfold safe_sub_t'.
+  unfold vsymbol in *.
+  destruct (aset_mem_dec (x, ty1) (tm_fv t2)); auto.
+  apply sub_t_typed; auto.
+  apply a_convert_t_ty; auto.
+Qed.
+
+Lemma safe_sub_f_typed' {gamma} (t1: term) (x: string) (f: formula) (ty1: vty):
+  term_has_type gamma t1 ty1 ->
+  formula_typed gamma f ->
+  formula_typed gamma (safe_sub_f' t1 (x, ty1) f).
+Proof.
+  intros Hty1 Hty2.
+  unfold safe_sub_f'.
+  unfold vsymbol in *.
+  destruct (aset_mem_dec (x, ty1) (fmla_fv f)); auto.
+  apply sub_f_typed; auto.
+  apply a_convert_f_typed; auto.
+Qed.
+
+Lemma safe_sub_t_fv' (tm: term) (x: vsymbol) (t: term):
+  aset_mem x (tm_fv t) ->
+  forall y,
+  aset_mem y (tm_fv (safe_sub_t' tm x t)) <->
+    (aset_mem y (tm_fv tm)) \/ ((aset_mem y (tm_fv t)) /\ y <> x).
+Proof.
+  intros.
+  unfold safe_sub_t'. unfold vsymbol in *.
+  destruct (aset_mem_dec x (tm_fv t)); try contradiction.
+  rewrite sub_t_fv.
+  + rewrite (alpha_equiv_t_fv t). reflexivity.
+    apply a_convert_t_equiv.
+  + rewrite (alpha_equiv_t_fv). apply H.
+    rewrite a_equiv_t_sym.
+    apply a_convert_t_equiv.
+  + intros.
+    intro C.
+    eapply (a_convert_t_bnd). 2: eauto. simpl_set; auto.
+Qed.
+
+Lemma safe_sub_f_fv' (tm: term) (x: vsymbol) (f: formula):
+  aset_mem x (fmla_fv f) ->
+  forall y,
+  aset_mem y (fmla_fv (safe_sub_f' tm x f)) <->
+    (aset_mem y (tm_fv tm)) \/ ((aset_mem y (fmla_fv f)) /\ y <> x).
+Proof.
+  intros.
+  unfold safe_sub_f'. unfold vsymbol in *.
+  destruct (aset_mem_dec x (fmla_fv f)); try contradiction.
+  rewrite sub_f_fv.
+  + rewrite (alpha_equiv_f_fv f). reflexivity.
+    apply a_convert_f_equiv.
+  + rewrite (alpha_equiv_f_fv). apply H.
+    rewrite a_equiv_f_sym.
+    apply a_convert_f_equiv.
+  + intros.
+    intro C.
+    eapply (a_convert_f_bnd). 2: eauto. simpl_set; auto.
+Qed.
+
+Lemma safe_sub_t_notin' (tm: term) (x: vsymbol) (t: term):
+  ~ aset_mem x (tm_fv t) ->
+  safe_sub_t' tm x t = t.
+Proof.
+  intros. unfold safe_sub_t'. unfold vsymbol in *.
+  destruct (aset_mem_dec x (tm_fv t)); auto; contradiction.
+Qed.
+
+Lemma safe_sub_f_notin' (tm: term) (x: vsymbol) (f: formula):
+  ~ aset_mem x (fmla_fv f) ->
+  safe_sub_f' tm x f = f.
+Proof.
+  intros. unfold safe_sub_f'. unfold vsymbol in *;
+  destruct (aset_mem_dec x (fmla_fv f)); auto; contradiction.
+Qed.
+
+Section Rep.
+
+Context {gamma: context} (gamma_valid: valid_context gamma)
+ {pd: pi_dom} {pdf: pi_dom_full gamma pd}
+  {vt: val_typevar} {pf: pi_funpred gamma_valid pd pdf}.
+
+Notation term_rep := (term_rep gamma_valid pd pdf vt pf).
+Notation formula_rep := (formula_rep gamma_valid pd pdf vt pf).
+
+Lemma safe_sub_t_rep' (t1 t2: term) (x: string)
+  (ty1 ty2: vty) (v: val_vars pd vt)
+  (Hty1: term_has_type gamma t1 ty1)
+  (Hty2: term_has_type gamma t2 ty2)
+  (Hty3: term_has_type gamma (safe_sub_t' t1 (x, ty1) t2) ty2):
+  term_rep v (safe_sub_t' t1 (x, ty1) t2) ty2 Hty3 =
+  term_rep (substi pd vt v (x, ty1)
+    (term_rep v t1 ty1 Hty1)) t2 ty2 Hty2.
+Proof.
+  revert Hty3.
+  unfold safe_sub_t'.
+  unfold vsymbol in *.
+  destruct (aset_mem_dec (x, ty1) (tm_fv t2)).
+  - intros. erewrite sub_t_rep with(Hty1:=Hty1).
+    + rewrite <- a_convert_t_rep; reflexivity.
+    + intros y Hiny1 Hiny2.
+      eapply a_convert_t_bnd. 2: eauto. simpl_set; auto.
+  - intros.
+    erewrite term_rep_irrel.
+    apply tm_change_vv.
+    intros.
+    unfold substi. vsym_eq x0 (x, ty1).
+Qed.
+
+Lemma safe_sub_f_rep' (t1: term) (x: string) (f: formula)
+  (ty1: vty) (v: val_vars pd vt)
+  (Hty1: term_has_type gamma t1 ty1)
+  (Hty2: formula_typed gamma f)
+  (Hty3: formula_typed gamma (safe_sub_f' t1 (x, ty1) f)):
+  formula_rep v (safe_sub_f' t1 (x, ty1) f) Hty3 =
+  formula_rep (substi pd vt v (x, ty1)
+    (term_rep v t1 ty1 Hty1)) f Hty2.
+Proof.
+  revert Hty3.
+  unfold safe_sub_f'.
+   unfold vsymbol in *.
+  destruct (aset_mem_dec (x, ty1) (fmla_fv f)).
+  - intros. erewrite sub_f_rep with(Hty1:=Hty1).
+    + rewrite <- a_convert_f_rep; reflexivity.
+    + intros y Hiny1 Hiny2. eapply a_convert_f_bnd; [| eauto]. simpl_set; auto.
+  - intros.
+    erewrite fmla_rep_irrel.
+    apply fmla_change_vv.
+    intros.
+    unfold substi. vsym_eq x0 (x, ty1).
+Qed.
+
+End Rep.
+
+
 Fixpoint elim_let_t (bt: bool) (bf: bool) (t: term) : term :=
   match t with
   | Tlet tm1 x tm2 => 
     if bt then
-    safe_sub_t (elim_let_t bt bf tm1) x (elim_let_t bt bf tm2)
+    safe_sub_t' (elim_let_t bt bf tm1) x (elim_let_t bt bf tm2)
     else Tlet (elim_let_t bt bf tm1) x (elim_let_t bt bf tm2)
   | Tfun f tys tms => Tfun f tys (map (elim_let_t bt bf) tms)
   | Tif f t1 t2 =>
@@ -34,7 +187,7 @@ with elim_let_f (bt: bool) (bf: bool) (f: formula) : formula :=
   | Fnot f => Fnot (elim_let_f bt bf f)
   | Flet tm1 v f =>
     if bf then
-    safe_sub_f (elim_let_t bt bf tm1) v (elim_let_f bt bf f)
+    safe_sub_f' (elim_let_t bt bf tm1) v (elim_let_f bt bf f)
     else Flet (elim_let_t bt bf tm1) v (elim_let_f bt bf f)
   | Fif f1 f2 f3 => Fif (elim_let_f bt bf f1) (elim_let_f bt bf f2)
     (elim_let_f bt bf f3)
@@ -63,7 +216,7 @@ Proof.
     constructor; auto.
   - destruct v as [x xty]; simpl in *.
     destruct bt. 
-    + apply safe_sub_t_typed; auto.
+    + apply safe_sub_t_typed'; auto.
     + constructor; auto.
   - constructor; auto.
     + intros x. rewrite in_map_iff.
@@ -86,7 +239,7 @@ Proof.
     constructor; auto.
   - destruct v as [x xty]; simpl in *.
     destruct bf. 
-    + apply safe_sub_f_typed; auto.
+    + apply safe_sub_f_typed'; auto.
     + constructor; auto.
   - constructor; auto.
     + intros x. rewrite in_map_iff.
@@ -119,9 +272,9 @@ Proof.
     + (*Need to know if var to sub appears freely in term or not*) 
       destruct (aset_mem_dec v  (tm_fv (elim_let_t true bf tm2))).
       * rewrite asubset_def in *. intros x.
-        rewrite safe_sub_t_fv; auto; simpl_set. intros;
+        rewrite safe_sub_t_fv'; auto; simpl_set. intros;
         destruct_all; auto.
-      * rewrite safe_sub_t_notin; auto.
+      * rewrite safe_sub_t_notin'; auto.
         rewrite asubset_def in *. intros.
         simpl_set.
         right. split; auto.
@@ -130,9 +283,9 @@ Proof.
   - destruct bf; simpl.
     + destruct (aset_mem_dec v  (fmla_fv (elim_let_f bt true f))).
       * rewrite asubset_def in *. intros x.
-        rewrite safe_sub_f_fv; auto; simpl_set. intros;
+        rewrite safe_sub_f_fv'; auto; simpl_set. intros;
         destruct_all; auto.
-      * rewrite safe_sub_f_notin; auto.
+      * rewrite safe_sub_f_notin'; auto.
         rewrite asubset_def in *. intros.
         simpl_set.
         right. split; auto.
@@ -176,7 +329,7 @@ Proof.
     apply H. apply nth_In; auto.
   - destruct bt.
     + destruct v as [x xty].
-      erewrite safe_sub_t_rep, H, H0.
+      erewrite safe_sub_t_rep', H, H0.
       reflexivity.
       Unshelve.
       all: inversion Hty1; subst;
@@ -213,7 +366,7 @@ Proof.
   - erewrite H; reflexivity.
   - destruct bf.
     + destruct v as [x xty].
-      erewrite safe_sub_f_rep, H, H0.
+      erewrite safe_sub_f_rep', H, H0.
       reflexivity.
       Unshelve.
       all: inversion Hty1; subst.
