src/proofs/ElimLet.v
@@ -18,7 +18,7 @@ Import MonadNotations.
 Local Open Scope errst_scope.
 
 (*Simple: eliminate all*)
-Check term_map.
+
 Definition elim_let_rewrite (t: term_c) : errState (CoqBigInt.t * hashcons_full) term_c :=
   term_map hashcons_full
   (*let is only interesting one*)
@@ -82,9 +82,8 @@ Definition lift_trans (f: task_hd -> errState (CoqBigInt.t * hashcons_full) task
 Definition elim_let : trans_errst task := lift_trans elim_let_aux.
 Set Bullet Behavior "Strict Subproofs".
 (*Soundness*)
-Require Import Task Relations ErrStateHoare StateInvar Soundness.
-Require Import eliminate_let.
-Check trans_errst.
+From Proofs Require Import Task eliminate_let Alpha.
+Require Import Relations ErrStateHoare StateInvar Soundness.
 
 (*TODO: move*)
 (*We can remove a pure proposition from a precondition of errst_spec*)
@@ -111,8 +110,6 @@ Proof.
   - intros Heval. exists f1. exists pr. auto.
   - intros [f2 [pr1 [Hsome Heval]]]. inversion Hsome; subst; auto.
 Qed.
-
-Require Import Alpha.
 
 (*Another attempt*)
 
@@ -255,6 +252,7 @@ Proof.
   intros [[Hlook1 Hlook2] | [Hlook1 [Hlook2 Heq]]] [[Hlook3 Hlook4] | [Hlook3 [Hlook4 Heq2]]]; subst; auto;
   rewrite Hlook1 in Hlook3; inversion Hlook3; auto.
 Qed.
+
 
 Lemma alpha_equiv_map_fv x y t1 f1:
   (forall m1 m2 t2 (Hv: amap_lookup m1 x = Some y) (Halpha: alpha_equiv_t m1 m2 t1 t2),
@@ -502,7 +500,36 @@ Proof.
     + apply alpha_equiv_var_sym; auto.
 Qed.
 
-(*TODO: formula version*)
+Lemma alpha_equiv_f_map_fv_aux m1 m2 f1 f2 x y
+  (Halpha: alpha_equiv_f m1 m2 f1 f2)
+  (Hvar: alpha_equiv_var m1 m2 x y):
+  aset_mem x (fmla_fv f1) -> aset_mem y (fmla_fv f2).
+Proof.
+  rewrite alpha_equiv_var_iff in Hvar.
+  destruct Hvar as [[Hlook1 Hlook2] | [Hlook1 [Hlook2 Heq]]]; subst.
+  - intros Hfv. apply alpha_equiv_f_map_fv with(x:=x)(y:=y) in Halpha; auto.
+    destruct_all; auto.
+  - apply alpha_f_fv_filter in Halpha.
+    apply (f_equal (fun s => aset_mem y s)) in Halpha.
+    apply ZifyClasses.eq_iff in Halpha.
+    rewrite !aset_mem_filter in Halpha.
+    intros Hmem.
+    apply Halpha. split; auto.
+    rewrite amap_mem_spec, Hlook1. auto.
+Qed.
+
+(*Then the iff (what we wanted to prove)*)
+Corollary alpha_equiv_f_map_fv_iff m1 m2 f1 f2 x y
+  (Halpha: alpha_equiv_f m1 m2 f1 f2)
+  (Hvar: alpha_equiv_var m1 m2 x y):
+  aset_mem x (fmla_fv f1) <-> aset_mem y (fmla_fv f2).
+Proof.
+  split.
+  - eapply alpha_equiv_f_map_fv_aux; eauto.
+  - apply alpha_equiv_f_map_fv_aux with (m1:=m2)(m2:=m1).
+    + rewrite alpha_equiv_f_sym; auto.
+    + apply alpha_equiv_var_sym; auto.
+Qed.
 
 (*General [same_in] - TODO: replace other version with this*)
 
@@ -584,6 +611,87 @@ with same_in_f (f1 f2: formula) (x y: vsymbol) : bool :=
   | _, _ => false
   end.
 
+(*Also generalization*)
+Lemma same_in_p_fv (p1 p2: pattern) x y:
+  same_in_p p1 p2 x y ->
+  aset_mem x (pat_fv p1) <-> aset_mem y (pat_fv p2).
+Proof.
+  revert p2. induction p1 as [x1| f1 tys1 ps1 IH | | p1 q1 IH1 IH2 | p1 x1 IH]; simpl; 
+  intros [x2| f2 tys2 ps2 | | p2 q2 | p2 x2]; try discriminate; simpl; try reflexivity;
+  intros Hsame.
+  - simpl_set. vsym_eq x1 x.
+    + vsym_eq x2 y; try discriminate. split; auto.
+    + vsym_eq x2 y; try discriminate. split; intros; subst; contradiction.
+  - rewrite andb_true in Hsame. destruct Hsame as [Hlen Hall].
+    apply Nat.eqb_eq in Hlen.
+    generalize dependent ps2. induction ps1 as [| p1 ps1 IHps]; intros [| p2 ps2]; try discriminate; auto.
+    simpl. intros Hlen. simpl_set_small. rewrite all2_cons, andb_true. intros [Hsamep Hallsame].
+    inversion IH as [| ? ? IH1 IH2]; subst.
+    rewrite IH1; auto. rewrite IHps; auto. auto.
+  - simpl_set_small. bool_hyps. rewrite (IH1 p2), (IH2 q2); auto.
+  - simpl_set_small. bool_hyps. rewrite (IH p2); auto.
+    apply or_iff_compat_l. vsym_eq x1 x.
+    + vsym_eq x2 y; try discriminate. split; auto.
+    + vsym_eq x2 y; try discriminate. split; intros; subst; contradiction.
+Qed. 
+
+Lemma same_in_p_notfv m1 m2 (p1 p2: pattern) x y:
+  ~ aset_mem x (pat_fv p1) ->
+  ~ aset_mem y (pat_fv p2) ->
+  or_cmp m1 m2 p1 p2 -> (*for shape*)
+  same_in_p p1 p2 x y.
+Proof.
+  revert p2. induction p1 as [x1| f1 tys1 ps1 IH | | p1 q1 IH1 IH2 | p1 x1 IH]; simpl; 
+  intros [x2| f2 tys2 ps2 | | p2 q2 | p2 x2]; try discriminate; simpl; try reflexivity;
+  intros Hn1 Hn2 Hor.
+  - rewrite aset_mem_singleton in Hn1, Hn2.
+    vsym_eq x1 x. vsym_eq x2 y.
+  - rewrite !andb_true in Hor. destruct Hor as [[[_ Hlenps] _] Hall].
+    rewrite Hlenps. simpl.
+    apply Nat.eqb_eq in Hlenps.
+    generalize dependent ps2. induction ps1 as [| p1 ps1 IHps]; intros [| p2 ps2]; try discriminate; auto.
+    simpl. revert Hn1. simpl. intros Hn1 Hn2.  rewrite all2_cons, andb_true.
+    intros Hlen [Hor1 Hallor]. simpl_set_small.
+    not_or Hn. inversion IH as [| ? ? IH1 IH2]; subst.
+    rewrite all2_cons. rewrite andb_true; split; auto.
+  - simpl_set_small. not_or Hn. bool_hyps. rewrite (IH1 p2), (IH2 q2); auto.
+  - simpl_set_small. bool_hyps. rewrite (IH p2); auto. simpl.
+    not_or Hn. vsym_eq x1 x. vsym_eq x2 y.
+Qed.
+
+(*Need something stronger: not just that they are both free or not but they map to each other*)
+(*NOTE: this is true but we don't need*)
+(* Lemma same_in_p_or_cmp (p1 p2: pattern) m1 m2 x y:
+  or_cmp m1 m2 p1 p2 ->
+  same_in_p p1 p2 x y ->
+  aset_mem x (pat_fv p1) ->
+  amap_lookup m1 x = Some y /\ amap_lookup m2 y = Some x.
+Proof.
+  revert p2. induction p1 as [x1| f1 tys1 ps1 IH | | p1 q1 IH1 IH2 | p1 x1 IH]; simpl; 
+  intros [x2| f2 tys2 ps2 | | p2 q2 | p2 x2]; try discriminate; simpl; try reflexivity;
+  intros Horcmp Hsame Hfv.
+  - unfold or_cmp_vsym in Horcmp. 
+    destruct (amap_lookup m1 x1) as [y1|] eqn : Hlook1; [|discriminate].
+    destruct (amap_lookup m2 x2) as [y2|] eqn : Hlook2; [|discriminate].
+    vsym_eq x2 y1; [|discriminate]. vsym_eq x1 y2; [|discriminate].
+    simpl_set. subst.
+    vsym_eq y2 y2. vsym_eq y1 y. discriminate.
+  - rewrite !andb_true in Hsame; rewrite !andb_true in Horcmp.
+    destruct Horcmp as [_ Hor]. destruct Hsame as [Hlen Hall].
+    apply Nat.eqb_eq in Hlen.
+    generalize dependent ps2. induction ps1 as [| p1 ps1 IHps]; intros [| p2 ps2]; try discriminate; auto.
+    simpl. rewrite !all2_cons, !andb_true. intros [Hor1 Hor2] Hlen [Hsamep Hallsame].
+    inversion IH as [| ? ? IH1 IH2]; subst.
+    simpl in Hfv. simpl_set_small. destruct Hfv as [Hx | Hx]; [eapply IH1 | eapply IHps]; eauto.
+  - simpl_set_small. bool_hyps. destruct Hfv; [apply (IH1 p2) | apply (IH2 q2)]; auto.
+  - simpl_set_small. bool_hyps. destruct Hfv; [apply (IH p2); auto|].
+    simpl_set. subst. vsym_eq x1 x1. vsym_eq x2 y; try discriminate.
+    unfold or_cmp_vsym in H2. 
+    destruct (amap_lookup m1 x1) as [y1|] eqn : Hlook1; [|discriminate].
+    destruct (amap_lookup m2 y) as [y2|] eqn : Hlook2; [|discriminate].
+    vsym_eq y y1; [|discriminate]. vsym_eq x1 y2. discriminate.
+Qed. *)
+
 Lemma keys_disj_equiv {A B: Type} `{countable.Countable A} (s: aset A) (m: amap A B):
   (forall x, aset_mem x s -> amap_lookup m x = None) <-> aset_disj (keys m) s.
 Proof.
@@ -617,6 +725,106 @@ Proof.
   - intros Hnotin Hmemx.
     specialize (Hnotin x). apply Hnotin; simpl_set; auto.
   - intros Hnotin y [Hmem Hmem']. simpl_set. subst. contradiction.
+Qed.
+
+Ltac split_disj_union :=
+  repeat match goal with
+  | H: aset_disj (aset_union ?s1 ?s2) ?s |- _ =>
+    let H1 := fresh "Hd" in
+    assert (H1:=H);
+    apply aset_disj_union_l in H; apply aset_disj_union_r in H1
+  end.
+
+Ltac solve_disj_union :=
+  split_disj_union; solve[auto].
+
+(*TODO: do single version*)
+
+Lemma amap_diff_aunion {A B: Type} `{countable.Countable A} (m1 m2: amap A B) (s: aset A):
+  amap_diff (aunion m1 m2) s = aunion (amap_diff m1 s) (amap_diff m2 s).
+Proof.
+  apply amap_ext.
+  intros x. rewrite aunion_lookup. destruct (aset_mem_dec x s).
+  - rewrite !amap_diff_in; auto.
+  - rewrite !amap_diff_notin; auto.
+    rewrite aunion_lookup. reflexivity.
+Qed.
+
+Lemma amap_diff_keys {A B: Type} `{countable.Countable A} (m1: amap A B):
+  amap_diff m1 (keys m1) = amap_empty.
+Proof.
+  apply amap_ext.
+  intros x. rewrite amap_empty_get.
+  destruct (aset_mem_dec x (keys m1)).
+  - apply amap_diff_in; auto.
+  - rewrite amap_diff_notin; auto. apply amap_lookup_none; auto.
+Qed.
+
+
+Lemma alpha_equiv_t_extra_union r1 r2 m1 m2 t1 t2:
+  aset_disj (keys r1) (tm_fv t1) ->
+  aset_disj (keys r2) (tm_fv t2) ->
+  alpha_equiv_t (aunion r1 m1) (aunion r2 m2) t1 t2 = alpha_equiv_t m1 m2 t1 t2.
+Proof.
+  intros Hdisj1 Hdisj2.
+  rewrite <- (alpha_equiv_t_diff) with (s:=keys r2); auto.
+  rewrite <- (alpha_equiv_t_diff _ _ (keys r2) m1 m2); auto.
+  (*And do other side*)
+  rewrite !(alpha_equiv_t_sym t1 t2).
+  rewrite <- (alpha_equiv_t_diff) with (s:=keys r1); auto.
+  rewrite <- (alpha_equiv_t_diff _ _ (keys r1) _ m1); auto.
+  (*Now prove maps equal*)
+  rewrite !amap_diff_aunion, !amap_diff_keys, !aunion_empty_l. reflexivity.
+Qed.
+
+(*Single version*)
+Lemma alpha_equiv_t_extra_var x y m1 m2 t1 t2:
+  ~ aset_mem x (tm_fv t1) ->
+  ~ aset_mem y (tm_fv t2) ->
+  alpha_equiv_t (amap_set m1 x y) (amap_set m2 y x) t1 t2 = alpha_equiv_t m1 m2 t1 t2.
+Proof.
+  intros Hmem1 Hmem2. rewrite !amap_set_aunion. apply alpha_equiv_t_extra_union;
+  rewrite !keys_singleton; apply aset_disj_singleton; auto.
+Qed.
+
+(*TODO: why didnt I prove in Alpha?*)
+Lemma alpha_equiv_f_diff (f1 f2: formula) (s: aset vsymbol) (m1 m2: amap vsymbol vsymbol)
+  (Hdisj: aset_disj s (fmla_fv f2)):
+  alpha_equiv_f m1 (amap_diff m2 s) f1 f2 = alpha_equiv_f m1 m2 f1 f2.
+Proof.
+  rewrite amap_diff_remove. rewrite aset_disj_equiv in Hdisj.
+  setoid_rewrite <- aset_to_list_in in Hdisj.
+  induction (aset_to_list s); simpl; auto.
+  simpl in Hdisj.
+  rewrite alpha_equiv_f_remove; auto.
+  - apply IHl. intros x [Hinx1 Hinx2]; apply (Hdisj x); auto.
+  - intros Hmem. apply (Hdisj a); auto. split; auto; simpl_set; auto.
+Qed.
+
+Lemma alpha_equiv_f_extra_union r1 r2 m1 m2 f1 f2:
+  aset_disj (keys r1) (fmla_fv f1) ->
+  aset_disj (keys r2) (fmla_fv f2) ->
+  alpha_equiv_f (aunion r1 m1) (aunion r2 m2) f1 f2 = alpha_equiv_f m1 m2 f1 f2.
+Proof.
+  intros Hdisj1 Hdisj2.
+  rewrite <- (alpha_equiv_f_diff) with (s:=keys r2); auto.
+  rewrite <- (alpha_equiv_f_diff _ _ (keys r2) m1 m2); auto.
+  (*And do other side*)
+  rewrite !(alpha_equiv_f_sym f1 f2).
+  rewrite <- (alpha_equiv_f_diff) with (s:=keys r1); auto.
+  rewrite <- (alpha_equiv_f_diff _ _ (keys r1) _ m1); auto.
+  (*Now prove maps equal*)
+  rewrite !amap_diff_aunion, !amap_diff_keys, !aunion_empty_l. reflexivity.
+Qed.
+
+(*Single version*)
+Lemma alpha_equiv_f_extra_var x y m1 m2 f1 f2:
+  ~ aset_mem x (fmla_fv f1) ->
+  ~ aset_mem y (fmla_fv f2) ->
+  alpha_equiv_f (amap_set m1 x y) (amap_set m2 y x) f1 f2 = alpha_equiv_f m1 m2 f1 f2.
+Proof.
+  intros Hmem1 Hmem2. rewrite !amap_set_aunion. apply alpha_equiv_f_extra_union;
+  rewrite !keys_singleton; apply aset_disj_singleton; auto.
 Qed.
 
 
@@ -658,7 +866,19 @@ Proof.
       simpl. (*Now prove from [amap_set]*)
       rewrite !alpha_equiv_var_iff in Halpha |- *.
       rewrite !amap_set_lookup_diff in Halpha; auto.
-  - admit.
+  - (*Tfun*)
+    intros f1 tys1 tms1 IHtms t2 m1 m2 Halpha2 Halpha Hsame Hd1 Hd2.
+    destruct t2 as [| | f2 tys2 tms2 | | | |]; try discriminate.
+    simpl.
+    destruct (funsym_eq_dec f1 f2); subst; [|discriminate]; simpl in Halpha. rewrite !length_map. 
+    destruct (Nat.eqb_spec (length tms1) (length tms2)) as [Hlen|]; [|discriminate]; simpl in *.
+    destruct (list_eq_dec _ tys1 tys2); [|discriminate]; subst. simpl in *.
+    rewrite all2_map.
+    generalize dependent tms2. induction tms1 as [| t1 tms1 IH]; intros [| t2 tms2]; try discriminate; simpl; auto.
+    rewrite !all2_cons, !andb_true.
+    intros [Halpha Hall] [Hsame1 Hsame2]. inversion IHtms as [| ? ? IH1 IH2]; subst; clear IHtms.
+    revert Hd1. simpl. rewrite !list_to_aset_app. intros Hd1 Hd2 Hlen.
+    split_disj_union. split; [apply IH1 | apply IH]; auto.
   - (*Tlet*)
     intros e1 v1 e2 IH1 IH2 t2 m1 m2 Halpha2 Halpha Hsame Hd1 Hd2.
     destruct t2 as [| | | e3 v2 e4 | | |]; try discriminate.
@@ -668,9 +888,8 @@ Proof.
     destruct Halpha as [[Hty Ha1] Ha2].
     rewrite !andb_true in Hsame. destruct Hsame as [[Hsame1 Heqvar] Hsame2].
     rewrite !list_to_aset_cons, !list_to_aset_app in Hd1, Hd2.
+    split_disj_union.
     apply IH1 in Ha1; auto.
-    2: { apply aset_disj_union_r, aset_disj_union_l in Hd1. auto. }
-    2: { apply aset_disj_union_r, aset_disj_union_l in Hd2. auto. }
     vsym_eq v1 x.
     + (*use same - crucial*)
       simpl in Heqvar. vsym_eq x x. vsym_eq v2 y. vsym_eq y y.
@@ -683,34 +902,433 @@ Proof.
       rewrite amap_set_reorder in Ha2; auto.
       rewrite (amap_set_reorder _ y v2) in Ha2; auto.
       apply IH2 in Ha2; auto.
-      2: { apply aset_disj_union_r, aset_disj_union_r in Hd1. auto. }
-      2: { apply aset_disj_union_r, aset_disj_union_r in Hd2. auto. }
       (*Now we can remove these vars because not free*)
-      assert (Hv1: ~ aset_mem v1 (tm_fv tm1)).
-      { apply aset_disj_union_l in Hd1. apply aset_disj_singleton; auto. }
-      assert (Hv2: ~ aset_mem v2 (tm_fv tm2)).
-      { apply aset_disj_union_l in Hd2. apply aset_disj_singleton; auto. }
-      (*separate lemma?*)
-      rewrite <- alpha_equiv_t_remove with (y2:=v2) in Halpha2 |- *; auto.
-      rewrite amap_remove_set_same.
-      (*And remove the other side*)
-      rewrite alpha_equiv_t_sym in Halpha2 |- *.
-      rewrite <- alpha_equiv_t_remove with (y2:=v1) in Halpha2 |- *; auto.
-      rewrite amap_remove_set_same.
-      apply Halpha2.
-  - 
-Admitted.
+      rewrite alpha_equiv_t_extra_var; auto; apply aset_disj_singleton; auto.
+  - (*Tif*)
+    intros f t1 t2 IH1 IH2 IH3 tm m1 m2 Halpha2 Halpha1 Hsame Hd1 Hd2.
+    destruct tm; try discriminate. simpl.
+    rewrite !andb_true in Halpha1, Hsame |- *.
+    destruct Halpha1 as [[Ha1 Ha2] Ha3]. destruct Hsame as [[Hs1 Hs2] Hs3].
+    simpl in Hd2. rewrite !list_to_aset_app in Hd1, Hd2. split_disj_union.
+    split_all; [apply IH1 | apply IH2 | apply IH3]; auto.
+  - (*Tmatch - generalizes let*)
+    intros t1 ty1 ps1 IHt1 IHps1 t2 m1 m2 Halpha2 Halpha1 Hsame Hd1 Hd2.
+    destruct t2 as [| | | | | t2 ty2 ps2 |]; try discriminate.
+    simpl in *. rewrite !length_map.
+    rewrite !andb_true in Halpha1, Hsame. (*Why doesn't this rewrite everything ugh*)
+    rewrite andb_true in Halpha1.
+    destruct Halpha1 as [[[Halpha1 Hlenps] Htyseq] Hall].
+    destruct Hsame as [[_ Hsame] Hallsame]. rewrite Hlenps.
+    apply Nat.eqb_eq in Hlenps. simpl_sumbool. simpl. rewrite !andb_true_r.
+    rewrite list_to_aset_app in Hd1, Hd2. split_disj_union.
+    rewrite andb_true; split; [auto|].
+    (*Inductive case*)
+    rewrite all2_map. simpl. clear IHt1 Halpha1 Hsame Hd1 Hd2 t1 t2 ty2.
+    rename Hd into Hd2. rename Hd0 into Hd1.
+    generalize dependent ps2. 
+    induction ps1 as [| [p1 t1] ps1 IH]; intros [| [p2 t2] ps2]; simpl; try discriminate; auto.
+    inversion IHps1 as [| ? ? IH1 IH2]; subst; clear IHps1. specialize (IH IH2). clear IH2.
+    rewrite !all2_cons. simpl.
+    intros Hlenps. destruct (a_equiv_p p1 p2) as [[r1 r2]|] eqn : Halphap; [|discriminate].
+    rewrite !andb_true.
+    intros [Halphat Hallalpha] [[Hsamep Hsamet] Hallsame].
+    revert Hd1. simpl. rewrite !list_to_aset_app. intros Hd1 Hd2. split_disj_union.
+    split; auto. (*IH case automatic*)
+    (*Prove head case - like let*)
+    assert (Hfviff:=Hsamep).
+    apply same_in_p_fv in Hfviff.
+    assert (Hvars:=Halphap).
+    apply a_equiv_p_vars_iff in Hvars. simpl in Hvars. destruct Hvars as [Hr1 Hr2].
+    (*Have to destruct - 2 cases*)
+    destruct (aset_mem_dec x (pat_fv p1) ) as [Hxfv | Hxfv];
+    destruct (aset_mem_dec y (pat_fv p2)) as [Hyfv | Hyfv]; [| tauto | tauto |]; simpl; rewrite Halphap.
+    + rewrite !aunion_set_infst in Halphat; auto.
+      * apply Hr2; auto.
+      * apply Hr1; auto.
+    + (*Idea: x not in r1 and y not in r2 so can rewrite as set*)
+      rewrite !aunion_set_not_infst in Halphat; [| rewrite Hr2; auto | rewrite Hr1; auto].
+      apply IH1 in Halphat; auto.
+      (*And now know from disj that we can remove r1 and r2 because no pat fv in tm1 or tm2 *)
+      rewrite alpha_equiv_t_extra_union; auto.
+      * (*Prove nothing in r1 in tm1 fvs*)
+        rewrite aset_to_list_to_aset_eq in Hd1.
+        replace (keys r1) with (pat_fv p1); auto.
+        apply aset_ext. intros v. rewrite <- Hr1. apply amap_mem_keys.
+      * (*and for r2*)
+        rewrite aset_to_list_to_aset_eq in Hd2.
+        replace (keys r2) with (pat_fv p2); auto.
+        apply aset_ext. intros v. rewrite <- Hr2. apply amap_mem_keys.
+  - (*Teps*)
+    intros f1 v1 IH t2 m1 m2 Halpha2 Halpha Hsame Hd1 Hd2.
+    destruct t2 as [| | | | | | f2 v2]; try discriminate.
+    simpl.
+    simpl in Hd2.
+    rewrite !andb_true in Halpha.
+    destruct Halpha as [Hty Ha].
+    rewrite !andb_true in Hsame. destruct Hsame as [Heqvar Hsame].
+    rewrite !list_to_aset_cons in Hd1, Hd2.
+    split_disj_union.
+    vsym_eq v1 x.
+    + simpl in Heqvar. vsym_eq x x. vsym_eq v2 y. vsym_eq y y. simpl.
+      rewrite !andb_true; split_all; auto.
+      (*Just setting x and y twice - same*)
+      rewrite !amap_set_twice in Ha. auto.
+    + simpl in Heqvar. vsym_eq x v1. vsym_eq v2 y. vsym_eq y v2. simpl.
+      (*Here, nothing is equal - we can reorder*)
+      rewrite !andb_true; split_all; auto.
+      rewrite amap_set_reorder in Ha; auto.
+      rewrite (amap_set_reorder _ y v2) in Ha; auto.
+      apply IH in Ha; auto.
+      rewrite alpha_equiv_t_extra_var; auto; apply aset_disj_singleton; auto.
+  - (*Fpred*)
+    intros p1 tys1 tms1 IHtms t2 m1 m2 Halpha2 Halpha Hsame Hd1 Hd2.
+    destruct t2 as [p2 tys2 tms2 | | | | | | | | |]; try discriminate.
+    simpl.
+    destruct (predsym_eq_dec p1 p2); subst; [|discriminate]; simpl in Halpha. rewrite !length_map. 
+    destruct (Nat.eqb_spec (length tms1) (length tms2)) as [Hlen|]; [|discriminate]; simpl in *.
+    destruct (list_eq_dec _ tys1 tys2); [|discriminate]; subst. simpl in *.
+    rewrite all2_map.
+    generalize dependent tms2. induction tms1 as [| t1 tms1 IH]; intros [| t2 tms2]; try discriminate; simpl; auto.
+    rewrite !all2_cons, !andb_true.
+    intros [Halpha Hall] [Hsame1 Hsame2]. inversion IHtms as [| ? ? IH1 IH2]; subst; clear IHtms.
+    revert Hd1. simpl. rewrite !list_to_aset_app. intros Hd1 Hd2 Hlen.
+    split_disj_union. split; [apply IH1 | apply IH]; auto.
+  - (*Fquant*)
+    intros q1 v1 f1 IH t2 m1 m2 Halpha2 Halpha Hsame Hd1 Hd2.
+    destruct t2 as [| q2 v2 f2 | | | | | | | |]; try discriminate.
+    simpl.
+    simpl in Hd2.
+    rewrite !andb_true in Halpha.
+    destruct Halpha as [[Hq Hty] Ha].
+    rewrite !andb_true in Hsame. destruct Hsame as [Heqvar Hsame].
+    rewrite !list_to_aset_cons in Hd1, Hd2.
+    split_disj_union.
+    vsym_eq v1 x.
+    + simpl in Heqvar. vsym_eq x x. vsym_eq v2 y. vsym_eq y y. simpl.
+      rewrite !andb_true; split_all; auto.
+      rewrite !amap_set_twice in Ha. auto.
+    + simpl in Heqvar. vsym_eq x v1. vsym_eq v2 y. vsym_eq y v2. simpl.
+      rewrite !andb_true; split_all; auto.
+      rewrite amap_set_reorder in Ha; auto.
+      rewrite (amap_set_reorder _ y v2) in Ha; auto.
+      apply IH in Ha; auto.
+      rewrite alpha_equiv_t_extra_var; auto; apply aset_disj_singleton; auto.
+  - (*Feq*)
+    intros ty1 t1 t2 IH1 IH2 tm m1 m2 Halpha2 Halpha1 Hsame Hd1 Hd2.
+    destruct tm; try discriminate. simpl.
+    rewrite !andb_true in Halpha1; rewrite !andb_true in Hsame; rewrite !andb_true.
+    destruct Halpha1 as [[ Htyeq Ha1] Ha2]. destruct Hsame as [Hs1 Hs2].
+    simpl in Hd2. rewrite !list_to_aset_app in Hd1, Hd2. split_disj_union. auto.
+  - (*Fbinop*)
+    intros b f1 f2 IH1 IH2 tm m1 m2 Halpha2 Halpha1 Hsame Hd1 Hd2.
+    destruct tm; try discriminate. simpl.
+    rewrite !andb_true in Halpha1; rewrite !andb_true in Hsame; rewrite !andb_true.
+    destruct Halpha1 as [[ Htyeq Ha1] Ha2]. destruct Hsame as [Hs1 Hs2].
+    simpl in Hd2. rewrite !list_to_aset_app in Hd1, Hd2. split_disj_union. auto.
+  - (*Fnot*)
+    intros f1 IH f2 m1 m2 Halpha2 Halpha1 Hsame. destruct f2; try discriminate.
+    simpl. intros. auto.
+  - (*Ftrue*) intros f2; intros. destruct f2; try discriminate. auto.
+  - (*Ffalse*) intros f2; intros. destruct f2; try discriminate. auto.
+  - (*Flet*) intros e1 v1 e2 IH1 IH2 t2 m1 m2 Halpha2 Halpha Hsame Hd1 Hd2.
+    destruct t2 as [| | | | | | | e3 v2 e4 | |]; try discriminate.
+    simpl.
+    simpl in Hd2.
+    rewrite !andb_true in Halpha.
+    destruct Halpha as [[Hty Ha1] Ha2].
+    rewrite !andb_true in Hsame. destruct Hsame as [[Hsame1 Heqvar] Hsame2].
+    rewrite !list_to_aset_cons, !list_to_aset_app in Hd1, Hd2.
+    split_disj_union.
+    apply IH1 in Ha1; auto.
+    vsym_eq v1 x.
+    + simpl in Heqvar. vsym_eq x x. vsym_eq v2 y. vsym_eq y y.
+      rewrite !andb_true; split_all; auto.
+      rewrite !amap_set_twice in Ha2. auto.
+    + simpl in Heqvar. vsym_eq x v1. vsym_eq v2 y. vsym_eq y v2.
+      rewrite !andb_true; split_all; auto.
+      rewrite amap_set_reorder in Ha2; auto.
+      rewrite (amap_set_reorder _ y v2) in Ha2; auto.
+      apply IH2 in Ha2; auto.
+      rewrite alpha_equiv_t_extra_var; auto; apply aset_disj_singleton; auto.
+  - (*Fif*)
+    intros f t1 t2 IH1 IH2 IH3 tm m1 m2 Halpha2 Halpha1 Hsame Hd1 Hd2.
+    destruct tm; try discriminate. simpl.
+    rewrite !andb_true in Halpha1, Hsame |- *.
+    destruct Halpha1 as [[Ha1 Ha2] Ha3]. destruct Hsame as [[Hs1 Hs2] Hs3].
+    simpl in Hd2. rewrite !list_to_aset_app in Hd1, Hd2. split_disj_union.
+    split_all; [apply IH1 | apply IH2 | apply IH3]; auto.
+  - (*Fmatch - exactly the same as Tmatch*)
+    intros t1 ty1 ps1 IHt1 IHps1 t2 m1 m2 Halpha2 Halpha1 Hsame Hd1 Hd2.
+    destruct t2 as [| | | | | | | | | t2 ty2 ps2]; try discriminate.
+    simpl in *. rewrite !length_map.
+    rewrite !andb_true in Halpha1, Hsame.
+    rewrite andb_true in Halpha1.
+    destruct Halpha1 as [[[Halpha1 Hlenps] Htyseq] Hall].
+    destruct Hsame as [[_ Hsame] Hallsame]. rewrite Hlenps.
+    apply Nat.eqb_eq in Hlenps. simpl_sumbool. simpl. rewrite !andb_true_r.
+    rewrite list_to_aset_app in Hd1, Hd2. split_disj_union.
+    rewrite andb_true; split; [auto|].
+    rewrite all2_map. simpl. clear IHt1 Halpha1 Hsame Hd1 Hd2 t1 t2 ty2.
+    rename Hd into Hd2. rename Hd0 into Hd1.
+    generalize dependent ps2. 
+    induction ps1 as [| [p1 t1] ps1 IH]; intros [| [p2 t2] ps2]; simpl; try discriminate; auto.
+    inversion IHps1 as [| ? ? IH1 IH2]; subst; clear IHps1. specialize (IH IH2). clear IH2.
+    rewrite !all2_cons. simpl.
+    intros Hlenps. destruct (a_equiv_p p1 p2) as [[r1 r2]|] eqn : Halphap; [|discriminate].
+    rewrite !andb_true.
+    intros [Halphat Hallalpha] [[Hsamep Hsamet] Hallsame].
+    revert Hd1. simpl. rewrite !list_to_aset_app. intros Hd1 Hd2. split_disj_union.
+    split; auto. assert (Hfviff:=Hsamep).
+    apply same_in_p_fv in Hfviff.
+    assert (Hvars:=Halphap).
+    apply a_equiv_p_vars_iff in Hvars. simpl in Hvars. destruct Hvars as [Hr1 Hr2].
+    destruct (aset_mem_dec x (pat_fv p1) ) as [Hxfv | Hxfv];
+    destruct (aset_mem_dec y (pat_fv p2)) as [Hyfv | Hyfv]; [| tauto | tauto |]; simpl; rewrite Halphap.
+    + rewrite !aunion_set_infst in Halphat; auto.
+      * apply Hr2; auto.
+      * apply Hr1; auto.
+    + rewrite !aunion_set_not_infst in Halphat; [| rewrite Hr2; auto | rewrite Hr1; auto].
+      apply IH1 in Halphat; auto.
+      rewrite alpha_equiv_t_extra_union; auto.
+      * rewrite aset_to_list_to_aset_eq in Hd1.
+        replace (keys r1) with (pat_fv p1); auto.
+        apply aset_ext. intros v. rewrite <- Hr1. apply amap_mem_keys.
+      * rewrite aset_to_list_to_aset_eq in Hd2.
+        replace (keys r2) with (pat_fv p2); auto.
+        apply aset_ext. intros v. rewrite <- Hr2. apply amap_mem_keys.
+Qed.
 
-(*TODO: prove rest of cases but should be doable*)
+Definition alpha_equiv_t_sub tm1 tm2 x y t1 t2 m1 m2 (Halpha1: alpha_equiv_t m1 m2 tm1 tm2)
+  (Halpha2: alpha_equiv_t (amap_set m1 x y) (amap_set m2 y x) t1 t2)
+  (Hsame: same_in_t t1 t2 x y)
+  (Hdisj1: aset_disj (list_to_aset (tm_bnd t1)) (tm_fv tm1))
+  (Hdisj2: aset_disj (list_to_aset (tm_bnd t2)) (tm_fv tm2)):
+  alpha_equiv_t m1 m2 (sub_t tm1 x t1) (sub_t tm2 y t2) :=
+  proj_tm (alpha_equiv_sub tm1 tm2 x y) t1 t2 m1 m2 Halpha1 Halpha2 Hsame Hdisj1 Hdisj2.
+
+Definition alpha_equiv_f_sub tm1 tm2 x y f1 f2 m1 m2 (Halpha1: alpha_equiv_t m1 m2 tm1 tm2)
+  (Halpha2: alpha_equiv_f (amap_set m1 x y) (amap_set m2 y x) f1 f2)
+  (Hsame: same_in_f f1 f2 x y)
+  (Hdisj1: aset_disj (list_to_aset (fmla_bnd f1)) (tm_fv tm1))
+  (Hdisj2: aset_disj (list_to_aset (fmla_bnd f2)) (tm_fv tm2)):
+  alpha_equiv_f m1 m2 (sub_f tm1 x f1) (sub_f tm2 y f2) :=
+  proj_fmla (alpha_equiv_sub tm1 tm2 x y) f1 f2 m1 m2 Halpha1 Halpha2 Hsame Hdisj1 Hdisj2.
+
+(*I hope this is true - if needed can assume in fv but that might make harder)*)
+(*NOT true if x or y can be bound
+  example: map x <-> z, terms x=x || forall x.x=x and z=z || forall y.y=y these are alpha equiv under x <-> z
+  but NOT same_in_t for x and z *)
+Lemma alpha_not_bnd_same x y t1 f1:
+  (forall m1 m2 t2 (Halpha: alpha_equiv_t (amap_set m1 x y) (amap_set m2 y x) t1 t2) 
+    (Hbnd1: ~ In x (tm_bnd t1)) (Hbnd2: ~ In y (tm_bnd t2)) (*TODO: do we need other?*)
+    (* (Hlook1: amap_lookup m1 x = Some y) *) (*(Hlook2: amap_lookup m2 y = Some x)*)
+    (* (Hfv1: aset_mem x (tm_fv t1)) *) (*(Hfv2: aset_mem y (tm_fv t2)*),
+    same_in_t t1 t2 x y) /\
+  (forall m1 m2 f2 (Halpha: alpha_equiv_f (amap_set m1 x y) (amap_set m2 y x) f1 f2) 
+    (Hbnd1: ~ In x (fmla_bnd f1)) (Hbnd2: ~ In y (fmla_bnd f2)),
+    same_in_f f1 f2 x y).
+Proof.
+  revert t1 f1; apply term_formula_ind; simpl; auto.
+  - intros c m1 m2 t2 Halpha. destruct t2; try discriminate. auto.
+  - (*Tvar*) intros v1 m1 m2 t2 Halpha Hbnd1. (*Hlook Hfv.*)
+    destruct t2 as [| v2 | | | | |]; try discriminate.
+    rewrite !alpha_equiv_var_iff in Halpha.
+    vsym_eq v1 x.
+    + rewrite !amap_set_lookup_same in Halpha. destruct Halpha as [[Hsome _] | [Hsome _]]; inversion Hsome; subst.
+      vsym_eq v2 v2.
+    + vsym_eq v2 y. rewrite !amap_set_lookup_same in Halpha.
+      destruct Halpha as [[_ Hsome] | [_ [Hsome _]]]; inversion Hsome; subst. contradiction.
+  - (*Tfun*)
+    intros f1 tys1 tms1 IH m1 m2 t2 Halpha Hbnd1 Hbnd2. destruct t2 as [| | f2 tys2 tms2 | | | | ]; try discriminate.
+    simpl. rewrite !andb_true in Halpha.
+    destruct Halpha as [[[ _ Hlen] _] Hall].
+    rewrite Hlen. simpl. apply Nat.eqb_eq in Hlen.
+    generalize dependent tms2. induction tms1 as [| t1 tms1 IHtms]; intros [| t2 tms2]; try discriminate; simpl; auto.
+    rewrite !all2_cons, !andb_true. intros Hlentms [Halpha Hall] Hbnd2. simpl in Hbnd1.
+    rewrite in_app_iff in Hbnd1, Hbnd2.
+    not_or Hbnd. inversion IH as [| ? ? IH1 IH2]; subst.
+    split; auto. eapply IH1; eauto.
+  - (*Tlet*)
+    intros tm1 v1 tm2 IH1 IH2 m1 m2 t2 Halpha Hbnd1 Hbnd2.
+    destruct t2 as [| | | tm3 v2 tm4 | | | ]; try discriminate.
+    rewrite !andb_true in Halpha |- *.
+    simpl in *. rewrite !in_app_iff in Hbnd1, Hbnd2. not_or Hbnd.
+    vsym_eq v1 x. vsym_eq v2 y.  
+    destruct Halpha as [[Htyeq Ha1] Ha2].
+    apply IH1 in Ha1; auto. rewrite Ha1. simpl.
+    split_all; auto.
+    (*not equal, so reorder*)
+    rewrite (amap_set_reorder _ x) in Ha2; auto.
+    rewrite (amap_set_reorder _ y) in Ha2; auto.
+    apply IH2 in Ha2; auto.
+  - (*Tif*)
+    intros f t1 t2 IH1 IH2 IH3 m1 m2 tm Halpha.
+    destruct tm; try discriminate; simpl in *.
+    rewrite !in_app_iff. intros Hbnd1 Hbnd2. not_or Hbnd.
+    rewrite !andb_true in Halpha |- *. destruct_all. split; eauto.
+  - (*Tmatch*)
+    intros tm1 ty1 ps1 IHtm1 IHps m1 m2 t2 Halpha.
+    destruct t2 as [| | | | | tm2 ty2 ps2 |]; try discriminate.
+    simpl in *. rewrite !in_app_iff. intros Hbnd1 Hbnd2.
+    rewrite !andb_true in Halpha.
+    destruct Halpha as [[[Halpha1 Hlenps] _] Hall].
+    rewrite Hlenps. simpl.
+    rewrite IHtm1 with (m1:=m1)(m2:=m2); auto. simpl.
+    not_or Hbnd. clear IHtm1 Halpha1 Hbnd2 Hbnd tm1 tm2 ty1 ty2.
+    rename Hbnd3 into Hbnd1. rename Hbnd0 into Hbnd2.
+    apply Nat.eqb_eq in Hlenps.
+    generalize dependent ps2.
+    induction ps1 as [| [p1 t1] ps1 IHps1]; intros [| [p2 t2] ps2]; try discriminate; auto.
+    simpl in *.
+    inversion IHps as [| ? ? IH1 IH2]; subst; clear IHps.
+    specialize (IHps1 IH2); clear IH2.
+    rewrite !all2_cons. simpl.
+    destruct (a_equiv_p p1 p2) as [[r1 r2]|] eqn : Halphap; [|discriminate].
+    intros Hlen. rewrite !andb_true. intros [Halphat Hall].
+    revert Hbnd1. rewrite !in_app_iff. intros Hbnd1 Hbnd2.
+    not_or Hbnd.
+    rewrite IHps1; auto. split; auto; clear IHps1 Hall.
+    (*Need to show if x and y not in free vars, then same_in_p*)
+    (*Again, need to flip set order*)
+    assert (Hvars:=Halphap).
+    apply a_equiv_p_vars_iff in Hvars. simpl in Hvars. destruct Hvars as [Hr1 Hr2].
+    rewrite aset_to_list_in in Hbnd1, Hbnd2.
+    rewrite !aunion_set_not_infst in Halphat; [| rewrite Hr2; auto | rewrite Hr1; auto].
+    apply IH1 in Halphat; auto. rewrite Halphat.
+    (*Lastly: not in fv so same_in_p trivially true*)
+    split; auto. apply a_equiv_p_or_cmp_iff in Halphap. destruct Halphap as [Hor _].
+    simpl in Hor. apply same_in_p_notfv with (m1:=r1)(m2:=r2); auto.
+  - (*Teps*)
+    intros f1 v1 IH m1 m2 t2 Halpha. destruct t2 as [| | | | | | f2 v2]; try discriminate.
+    simpl. intros. not_or Hbnd. vsym_eq v1 x. vsym_eq v2 y. simpl.
+    rewrite andb_true in Halpha. destruct Halpha as [_ Ha].
+    rewrite (amap_set_reorder _ x) in Ha; auto.
+    rewrite (amap_set_reorder _ y) in Ha; auto.
+    apply IH in Ha; auto.
+  - (*Fpred*)
+    intros p1 tys1 tms1 IH m1 m2 t2 Halpha Hbnd1 Hbnd2. destruct t2 as [p2 tys2 tms2 | | | | | | | | |]; try discriminate.
+    simpl. rewrite !andb_true in Halpha.
+    destruct Halpha as [[[ _ Hlen] _] Hall].
+    rewrite Hlen. simpl. apply Nat.eqb_eq in Hlen.
+    generalize dependent tms2. induction tms1 as [| t1 tms1 IHtms]; intros [| t2 tms2]; try discriminate; simpl; auto.
+    rewrite !all2_cons, !andb_true. intros Hlentms [Halpha Hall] Hbnd2. simpl in Hbnd1.
+    rewrite in_app_iff in Hbnd1, Hbnd2.
+    not_or Hbnd. inversion IH as [| ? ? IH1 IH2]; subst.
+    split; auto. eapply IH1; eauto.
+  - (*Fquant*)
+    intros q1 v1 f1 IH m1 m2 t2 Halpha. destruct t2 as [| q2 v2 f2 | | | | | | | | ]; try discriminate.
+    simpl. intros. not_or Hbnd. vsym_eq v1 x. vsym_eq v2 y. simpl.
+    rewrite andb_true in Halpha. destruct Halpha as [_ Ha].
+    rewrite (amap_set_reorder _ x) in Ha; auto.
+    rewrite (amap_set_reorder _ y) in Ha; auto.
+    apply IH in Ha; auto.
+  - (*Feq*)
+    intros ty t1 t2 IH1 IH2 m1 m2 f2 Halpha. destruct f2; try discriminate. simpl.
+    rewrite !in_app_iff. intros. not_or Hbnd. rewrite !andb_true in Halpha.
+    destruct Halpha as [[_ Ha1] Ha2]. rewrite andb_true; split; [eapply IH1 | eapply IH2]; eauto.
+  - (*Fbinop*)
+    intros b f1 f2 IH1 IH2 m1 m2 fm Halpha. destruct fm; try discriminate. simpl.
+    rewrite !in_app_iff. intros. not_or Hbnd. rewrite !andb_true in Halpha.
+    destruct Halpha as [[_ Ha1] Ha2]. rewrite andb_true; split; [eapply IH1 | eapply IH2]; eauto.
+  - (*Fnot*)
+    intros f IH m1 m2 f2 Halpha. destruct f2; try discriminate. simpl. intros; eauto.
+  - (*Flet*)
+    intros tm1 v1 tm2 IH1 IH2 m1 m2 f2 Halpha Hbnd1 Hbnd2.
+    destruct f2 as [| | | | | | | tm3 v2 tm4 | | ]; try discriminate.
+    rewrite !andb_true in Halpha |- *.
+    simpl in *. rewrite !in_app_iff in Hbnd1, Hbnd2. not_or Hbnd.
+    vsym_eq v1 x. vsym_eq v2 y.  
+    destruct Halpha as [[Htyeq Ha1] Ha2].
+    apply IH1 in Ha1; auto. rewrite Ha1. simpl.
+    split_all; auto.
+    rewrite (amap_set_reorder _ x) in Ha2; auto.
+    rewrite (amap_set_reorder _ y) in Ha2; auto.
+    apply IH2 in Ha2; auto.
+  - (*Fif*)
+    intros f t1 t2 IH1 IH2 IH3 m1 m2 tm Halpha.
+    destruct tm; try discriminate; simpl in *.
+    rewrite !in_app_iff. intros Hbnd1 Hbnd2. not_or Hbnd.
+    rewrite !andb_true in Halpha |- *. destruct_all. split; eauto.
+  - (*Fmatch*)
+    intros tm1 ty1 ps1 IHtm1 IHps m1 m2 t2 Halpha.
+    destruct t2 as [| | | | |  | | | | tm2 ty2 ps2]; try discriminate.
+    simpl in *. rewrite !in_app_iff. intros Hbnd1 Hbnd2.
+    rewrite !andb_true in Halpha.
+    destruct Halpha as [[[Halpha1 Hlenps] _] Hall].
+    rewrite Hlenps. simpl.
+    rewrite IHtm1 with (m1:=m1)(m2:=m2); auto. simpl.
+    not_or Hbnd. clear IHtm1 Halpha1 Hbnd2 Hbnd tm1 tm2 ty1 ty2.
+    rename Hbnd3 into Hbnd1. rename Hbnd0 into Hbnd2.
+    apply Nat.eqb_eq in Hlenps.
+    generalize dependent ps2.
+    induction ps1 as [| [p1 t1] ps1 IHps1]; intros [| [p2 t2] ps2]; try discriminate; auto.
+    simpl in *.
+    inversion IHps as [| ? ? IH1 IH2]; subst; clear IHps.
+    specialize (IHps1 IH2); clear IH2.
+    rewrite !all2_cons. simpl.
+    destruct (a_equiv_p p1 p2) as [[r1 r2]|] eqn : Halphap; [|discriminate].
+    intros Hlen. rewrite !andb_true. intros [Halphat Hall].
+    revert Hbnd1. rewrite !in_app_iff. intros Hbnd1 Hbnd2.
+    not_or Hbnd.
+    rewrite IHps1; auto. split; auto; clear IHps1 Hall.
+    assert (Hvars:=Halphap).
+    apply a_equiv_p_vars_iff in Hvars. simpl in Hvars. destruct Hvars as [Hr1 Hr2].
+    rewrite aset_to_list_in in Hbnd1, Hbnd2.
+    rewrite !aunion_set_not_infst in Halphat; [| rewrite Hr2; auto | rewrite Hr1; auto].
+    apply IH1 in Halphat; auto. rewrite Halphat.
+    split; auto. apply a_equiv_p_or_cmp_iff in Halphap. destruct Halphap as [Hor _].
+    simpl in Hor. apply same_in_p_notfv with (m1:=r1)(m2:=r2); auto.
+Qed.
+
+Definition alpha_not_bnd_same_in_t x y t1 t2 m1 m2 
+  (Halpha: alpha_equiv_t (amap_set m1 x y) (amap_set m2 y x) t1 t2) 
+  (Hbnd1: ~ In x (tm_bnd t1)) (Hbnd2: ~ In y (tm_bnd t2)):
+  same_in_t t1 t2 x y :=
+  proj_tm (alpha_not_bnd_same x y) t1 m1 m2 t2 Halpha Hbnd1 Hbnd2.
+
+Definition alpha_not_bnd_same_in_f x y f1 f2 m1 m2 
+  (Halpha: alpha_equiv_f (amap_set m1 x y) (amap_set m2 y x) f1 f2) 
+  (Hbnd1: ~ In x (fmla_bnd f1)) (Hbnd2: ~ In y (fmla_bnd f2)):
+  same_in_f f1 f2 x y :=
+  proj_fmla (alpha_not_bnd_same x y) f1 m1 m2 f2 Halpha Hbnd1 Hbnd2.
+
+(*And we can combine the two results: instead of assuming [same_in_t], we can just
+  assume we the variable we substitute for is not bound*)
+
+Corollary alpha_equiv_t_sub_not_bnd (tm1 tm2 : term) (x y : vsymbol) (t1 t2 : term) (m1 m2 : amap vsymbol vsymbol)
+  (Halpha1: alpha_equiv_t m1 m2 tm1 tm2)
+  (Halpha2: alpha_equiv_t (amap_set m1 x y) (amap_set m2 y x) t1 t2)
+  (Hbnd1: ~ In x (tm_bnd t1)) (Hbnd2: ~ In y (tm_bnd t2))
+  (Hdisj1: aset_disj (list_to_aset (tm_bnd t1)) (tm_fv tm1))
+  (Hdisj2: aset_disj (list_to_aset (tm_bnd t2)) (tm_fv tm2)):
+  alpha_equiv_t m1 m2 (sub_t tm1 x t1) (sub_t tm2 y t2).
+Proof.
+  apply alpha_equiv_t_sub; auto.
+  eapply alpha_not_bnd_same_in_t; eauto.
+Qed.
+
+Corollary alpha_equiv_f_sub_not_bnd (tm1 tm2 : term) (x y : vsymbol) (f1 f2 : formula) (m1 m2 : amap vsymbol vsymbol)
+  (Halpha1: alpha_equiv_t m1 m2 tm1 tm2)
+  (Halpha2: alpha_equiv_f (amap_set m1 x y) (amap_set m2 y x) f1 f2)
+  (Hbnd1: ~ In x (fmla_bnd f1)) (Hbnd2: ~ In y (fmla_bnd f2))
+  (Hdisj1: aset_disj (list_to_aset (fmla_bnd f1)) (tm_fv tm1))
+  (Hdisj2: aset_disj (list_to_aset (fmla_bnd f2)) (tm_fv tm2)):
+  alpha_equiv_f m1 m2 (sub_f tm1 x f1) (sub_f tm2 y f2).
+Proof.
+  apply alpha_equiv_f_sub; auto.
+  eapply alpha_not_bnd_same_in_f; eauto.
+Qed.
 
 
-(*TODO: need type equality?*)
+
+(*Cannot use [safe_sub_t] because if we don't alpha convert, dont have
+  the tm_bnd condition (and don't have [same_in_t] necessarily*)
 Lemma safe_sub_t_alpha m1 m2 v1 v2 t1 t2 t3 t4
   (Halpha1: alpha_equiv_t m1 m2 t1 t2)
   (Halpha2: alpha_equiv_t (amap_set m1 v1 v2) (amap_set m2 v2 v1) t3 t4):
-  alpha_equiv_t m1 m2 (safe_sub_t t1 v1 t3) (safe_sub_t t2 v2 t4).
+  alpha_equiv_t m1 m2 (safe_sub_t' t1 v1 t3) (safe_sub_t' t2 v2 t4).
 Proof.
-  unfold safe_sub_t.
+  unfold safe_sub_t'.
   (*Why we needed the previous: v1 in fv of t3 iff v2 in fv of t4*)
   assert (Hfvs: aset_mem v1 (tm_fv t3) <-> aset_mem v2 (tm_fv t4)). {
     eapply alpha_equiv_t_map_fv_iff; eauto.
@@ -719,33 +1337,12 @@ Proof.
   (*Annoyingly, have to destruct by cases*)
   destruct (aset_mem_dec v1 (tm_fv t3)) as [Hv1 | Hv1]; 
   destruct (aset_mem_dec v2 (tm_fv t4)) as [Hv2 | Hv2]; [| tauto | tauto |].
-  2: {
-    (*In this case, can remove these from the map because free vars not present*)
-    rewrite <- alpha_equiv_t_remove with (y2:=v2) in Halpha2 |- *; auto.
-    rewrite amap_remove_set_same in Halpha2.
-    (*And remove the other side*)
-    rewrite alpha_equiv_t_sym in Halpha2 |- *.
-    rewrite <- alpha_equiv_t_remove with (y2:=v1) in Halpha2 |- *; auto.
-    rewrite amap_remove_set_same in Halpha2.
-    apply Halpha2.
-  }
-  (*It doesn't actually matter which we substitute. But the result is alpha equivalent to t3*)
-  set (t3':=(if existsb (fun x : vsymbol => in_bool vsymbol_eq_dec x (tm_bnd t3)) (aset_to_list (tm_fv t1))
-      then a_convert_t t3 (tm_fv t1)
-      else t3)).
-  set (t4':=(if existsb (fun x : vsymbol => in_bool vsymbol_eq_dec x (tm_bnd t4)) (aset_to_list (tm_fv t2))
-      then a_convert_t t4 (tm_fv t2)
-      else t4)).
-  assert (Ht3: a_equiv_t t3 t3'). {
-    unfold t3'. destruct (existsb _). 
-    - apply a_convert_t_equiv.
-    - apply a_equiv_t_refl.
-  }
-  assert (Ht4: a_equiv_t t4 t4'). {
-    unfold t4'. clear. destruct (existsb _). 
-    - apply a_convert_t_equiv.
-    - apply a_equiv_t_refl.
-  }
+  2: { (*In this case, can remove these from the map because free vars not present*) 
+    rewrite alpha_equiv_t_extra_var in Halpha2; auto. }
+  set (t3':=(a_convert_t t3 (aset_union (tm_fv t1) (tm_fv t3)))).
+  set (t4':=(a_convert_t t4 (aset_union (tm_fv t2) (tm_fv t4)))).
+  assert (Ht3: a_equiv_t t3 t3') by apply a_convert_t_equiv.
+  assert (Ht4: a_equiv_t t4 t4') by apply a_convert_t_equiv.
   assert (Ht34: alpha_equiv_t (amap_set m1 v1 v2) (amap_set m2 v2 v1) t3' t4'). {
     pose proof (alpha_equiv_t_trans t3' t3 t4' amap_empty amap_empty (amap_set m1 v1 v2) (amap_set m2 v2 v1)) as Htrans.
     forward Htrans.
@@ -757,24 +1354,61 @@ Proof.
     }
     rewrite alpha_comp_empty_r, alpha_comp_empty_l in Htrans. auto.
   }
-  (*Should be provable with previous*)
-Admitted.
+  (*Prove disj*)
+  assert (Hdisj1: aset_disj (list_to_aset (tm_bnd t3')) (tm_fv t1)).
+  { unfold t3'. clear. rewrite aset_disj_equiv. intros x [Hx1 Hx2].
+    apply (a_convert_t_bnd t3 (aset_union (tm_fv t1) (tm_fv t3)) x); auto; simpl_set; auto. }
+  assert (Hdisj2: aset_disj (list_to_aset (tm_bnd t4')) (tm_fv t2)).
+  { unfold t4'. clear. rewrite aset_disj_equiv. intros x [Hx1 Hx2].
+    apply (a_convert_t_bnd t4 (aset_union (tm_fv t2) (tm_fv t4)) x); auto; simpl_set; auto. }
+  (*Now use previous*)
+  apply alpha_equiv_t_sub_not_bnd; auto.
+  - intros Hinv. apply a_convert_t_bnd in Hinv; auto. simpl_set; auto.
+  - intros Hinv. apply a_convert_t_bnd in Hinv; auto. simpl_set; auto.
+Qed.
 
-
-
-(* alpha_equiv_sub_var_t_full:
-  forall (t t2 : term) (x y : vsymbol) (m1 m2 : amap vsymbol vsymbol),
-  snd x = snd y ->
-  ~ In y (tm_bnd t2) ->
-  ~ aset_mem y (tm_fv t2) ->
-  same_in_t t t2 x ->
-  ~ amap_mem y m2 ->
-  alpha_equiv_t m1 m2 t t2 -> alpha_equiv_t (amap_set m1 x y) (amap_set m2 y x) t (sub_var_t x y t2)
- *)
-
-(*TODO: generalize, define previous by this*)
-
-
+Lemma safe_sub_f_alpha m1 m2 v1 v2 t1 t2 f3 f4
+  (Halpha1: alpha_equiv_t m1 m2 t1 t2)
+  (Halpha2: alpha_equiv_f (amap_set m1 v1 v2) (amap_set m2 v2 v1) f3 f4):
+  alpha_equiv_f m1 m2 (safe_sub_f' t1 v1 f3) (safe_sub_f' t2 v2 f4).
+Proof.
+  unfold safe_sub_f'.
+  assert (Hfvs: aset_mem v1 (fmla_fv f3) <-> aset_mem v2 (fmla_fv f4)). {
+    eapply alpha_equiv_f_map_fv_iff; eauto.
+    rewrite alpha_equiv_var_iff. rewrite !amap_set_lookup_same. auto.
+  }
+  (*Annoyingly, have to destruct by cases*)
+  destruct (aset_mem_dec v1 (fmla_fv f3)) as [Hv1 | Hv1]; 
+  destruct (aset_mem_dec v2 (fmla_fv f4)) as [Hv2 | Hv2]; [| tauto | tauto |].
+  2: { (*In this case, can remove these from the map because free vars not present*) 
+    rewrite alpha_equiv_f_extra_var in Halpha2; auto. }
+  set (f3':=(a_convert_f f3 (aset_union (tm_fv t1) (fmla_fv f3)))).
+  set (f4':=(a_convert_f f4 (aset_union (tm_fv t2) (fmla_fv f4)))).
+  assert (Ht3: a_equiv_f f3 f3') by apply a_convert_f_equiv.
+  assert (Ht4: a_equiv_f f4 f4') by apply a_convert_f_equiv.
+  assert (Ht34: alpha_equiv_f (amap_set m1 v1 v2) (amap_set m2 v2 v1) f3' f4'). {
+    pose proof (alpha_equiv_f_trans f3' f3 f4' amap_empty amap_empty (amap_set m1 v1 v2) (amap_set m2 v2 v1)) as Htrans.
+    forward Htrans.
+    { rewrite alpha_equiv_f_sym; auto. }
+    forward Htrans.
+    { pose proof (alpha_equiv_f_trans f3 f4 f4' (amap_set m1 v1 v2) (amap_set m2 v2 v1) amap_empty amap_empty Halpha2 Ht4) 
+      as Htrans1.
+      rewrite alpha_comp_empty_r, alpha_comp_empty_l in Htrans1. auto.
+    }
+    rewrite alpha_comp_empty_r, alpha_comp_empty_l in Htrans. auto.
+  }
+  (*Prove disj*)
+  assert (Hdisj1: aset_disj (list_to_aset (fmla_bnd f3')) (tm_fv t1)).
+  { unfold f3'. clear. rewrite aset_disj_equiv. intros x [Hx1 Hx2].
+    apply (a_convert_f_bnd f3 (aset_union (tm_fv t1) (fmla_fv f3)) x); auto; simpl_set; auto. }
+  assert (Hdisj2: aset_disj (list_to_aset (fmla_bnd f4')) (tm_fv t2)).
+  { unfold f4'. clear. rewrite aset_disj_equiv. intros x [Hx1 Hx2].
+    apply (a_convert_f_bnd f4 (aset_union (tm_fv t2) (fmla_fv f4)) x); auto; simpl_set; auto. }
+  (*Now use previous*)
+  apply alpha_equiv_f_sub_not_bnd; auto.
+  - intros Hinv. apply a_convert_f_bnd in Hinv; auto. simpl_set; auto.
+  - intros Hinv. apply a_convert_f_bnd in Hinv; auto. simpl_set; auto.
+Qed.
 
 
 Lemma elim_let_alpha_equiv b1 b2 t1 f1:
@@ -804,42 +1438,89 @@ Proof.
     2: { rewrite Htyeq. destruct (vty_eq_dec _ _); simpl; auto. rewrite andb_true; split; auto. }
     apply IH1 in Halpha1.
     apply IH2 in Halpha2.
-    set (t1 := (elim_let_t true b2 tm1) ) in *.
-    set (t2:=(elim_let_t true b2 e1)) in *.
-    set (t3:=(elim_let_t true b2 tm2)) in *.
-    set (t4:=(elim_let_t true b2 e3)) in *.
-    (*Could assume: tm1 and tm2 with m3 and m4, then t1 and t2 with m1 U m3 and m2 U m4
-      then want to show safe_sub_t with  *)
     apply safe_sub_t_alpha; auto.
-Admitted.
+  - (*Tif*)
+    intros f1 t1 t2 IH1 IH2 IH3 m1 m2 tm Halpha.
+    destruct tm; try discriminate. simpl. rewrite !andb_true in Halpha |- *.
+    destruct Halpha as [[Ha1 Ha2] Ha3]. split_all; auto.
+  - (*Tmatch*)
+    intros tm1 ty1 ps1 IHtm IHps m1 m2 t2 Halpha.
+    destruct t2 as [| | | | | tm2 tys2 ps2 |]; try discriminate. simpl in *.
+    rewrite !length_map.
+    rewrite !andb_true in Halpha. destruct Halpha as [[[Halphat Hlenps] Htys] Hall].
+    rewrite Hlenps, Htys, !andb_true_r.
+    rewrite IHtm; auto. simpl. clear IHtm Halphat Htys tm1 tm2 ty1 tys2.
+    apply Nat.eqb_eq in Hlenps.
+    generalize dependent ps2. 
+    induction ps1 as [| [p1 t1] ps1 IHps1]; intros [| [p2 t2] ps2]; simpl; try discriminate; auto.
+    intros Hlenps. rewrite !all2_cons. simpl.
+    destruct (a_equiv_p p1 p2) as [[r1 r2]|] eqn : Halphap; [|discriminate].
+    rewrite andb_true. intros [Halphat Hall].
+    inversion IHps as [|? ? IH1 IH2]; subst; clear IHps. specialize (IHps1 IH2); clear IH2.
+    rewrite IHps1; auto. clear IHps1 Hall. rewrite andb_true_r. auto.
+  - (*Teps*)
+    intros f1 v1 IH m1 m2 t2 Halpha. destruct t2; try discriminate. simpl.
+    rewrite andb_true in Halpha |- *. destruct_all; split; auto.
+  - (*Fpred*)
+    intros p1 tys1 tms1 IH m1 m2 t2 Halpha. destruct t2 as [p2 tys2 tms2 | | | | | | | | | ]; try discriminate.
+    simpl. destruct (predsym_eq_dec p1 p2); subst; [|discriminate]; simpl in Halpha. simpl.
+    rewrite !length_map. destruct (Nat.eqb_spec (length tms1) (length tms2)) as [Hlen|]; [|discriminate]; simpl in *.
+    destruct (list_eq_dec _ tys1 tys2); [|discriminate]; subst. simpl in *.
+    rewrite !all2_map.
+    generalize dependent tms2. induction tms1 as [| t1 tms1 IHtms]; intros [| t2 tms2]; try discriminate; simpl; auto.
+    rewrite !all2_cons, !andb_true.
+    intros [Halpha Hall] Hlentms. inversion IH as [| ? ? IH1 IH2]; subst.
+    split; auto.
+  - (*Fquant*)
+    intros q1 v1 f1 IH m1 m2 t2 Halpha. destruct t2; try discriminate. simpl.
+    rewrite andb_true in Halpha |- *. destruct_all; split; auto.
+  - (*Feq*) intros ty t1 t2 IH1 IH2 m1 m2 f2 Halpha. destruct f2; try discriminate. simpl.
+    bool_hyps. bool_to_prop. split_all; auto; [apply IH1 | apply IH2]; auto.
+  - (*Fpred*) intros b t1 t2 IH1 IH2 m1 m2 f2 Halpha. destruct f2; try discriminate. simpl.
+    bool_hyps. bool_to_prop. split_all; auto; [apply IH1 | apply IH2]; auto.
+  - (*Fnot*) intros f IH m1 m2 f2 Halpha. destruct f2; try discriminate; simpl; auto.
+  - (*Ftrue*) intros _ _ f2 Halpha; destruct f2; try discriminate; auto.
+  - (*Ffalse*) intros _ _ f2 Halpha; destruct f2; try discriminate; auto.
+  - (*Flet*) intros tm1 v1 tm2 IH1 IH2 m1 m2 t2 Halpha. destruct t2 as [| | | | | | | e1 v2 e3 | | ]; try discriminate.
+    destruct (vty_eq_dec (snd v1) (snd v2)) as [Htyeq|]; [|discriminate]; simpl in Halpha.
+    rewrite andb_true in Halpha. destruct Halpha as [Halpha1 Halpha2].
+    destruct b2; simpl; auto.
+    2: { rewrite Htyeq. destruct (vty_eq_dec _ _); simpl; auto. rewrite andb_true; split; auto. }
+    apply IH1 in Halpha1.
+    apply IH2 in Halpha2.
+    apply safe_sub_f_alpha; auto.
+  - (*Fif*)
+    intros f1 t1 t2 IH1 IH2 IH3 m1 m2 tm Halpha.
+    destruct tm; try discriminate. simpl. rewrite !andb_true in Halpha |- *.
+    destruct Halpha as [[Ha1 Ha2] Ha3]. split_all; auto.
+  - (*Fmatch*)
+    intros tm1 ty1 ps1 IHtm IHps m1 m2 t2 Halpha.
+    destruct t2 as [| | | | | | | | | tm2 tys2 ps2]; try discriminate. simpl in *.
+    rewrite !length_map.
+    rewrite !andb_true in Halpha. destruct Halpha as [[[Halphat Hlenps] Htys] Hall].
+    rewrite Hlenps, Htys, !andb_true_r.
+    rewrite IHtm; auto. simpl. clear IHtm Halphat Htys tm1 tm2 ty1 tys2.
+    apply Nat.eqb_eq in Hlenps.
+    generalize dependent ps2. 
+    induction ps1 as [| [p1 t1] ps1 IHps1]; intros [| [p2 t2] ps2]; simpl; try discriminate; auto.
+    intros Hlenps. rewrite !all2_cons. simpl.
+    destruct (a_equiv_p p1 p2) as [[r1 r2]|] eqn : Halphap; [|discriminate].
+    rewrite andb_true. intros [Halphat Hall].
+    inversion IHps as [|? ? IH1 IH2]; subst; clear IHps. specialize (IHps1 IH2); clear IH2.
+    rewrite IHps1; auto. clear IHps1 Hall. rewrite andb_true_r. auto.
+Qed.
 
+(*Only need f version*)
 
-    Search elim_let_t tm_fv.
+Definition elim_let_f_alpha_equiv b1 b2 f1 f2 m1 m2 (Halpha: alpha_equiv_f m1 m2 f1 f2):
+  alpha_equiv_f m1 m2 (elim_let_f b1 b2 f1) (elim_let_f b1 b2 f2) :=
+  proj_fmla (elim_let_alpha_equiv b1 b2) f1 m1 m2 f2 Halpha.
 
+(*And corollary for empty maps*)
+Definition elim_let_f_a_equiv b1 b2 f1 f2 (Halpha: a_equiv_f f1 f2):
+  a_equiv_f (elim_let_f b1 b2 f1) (elim_let_f b1 b2 f2) :=
+  elim_let_f_alpha_equiv b1 b2 f1 f2 amap_empty amap_empty Halpha.
 
-
-    unfold safe_sub_t.
-    (*TODO: should do [safe_sub_t] in different lemma*)
-    (*oh btw I already have the free var optimization but only in [safe_sub_t]*)
-
-    Search alpha_equiv_t safe_sub_t.
- 
-
-    Search all2 combine.
-    Search all2 "impl".
-
-
-
-
-all2_Forall2
-    Search all2 Forall2.
-
-
- auto.
-    Search all2 map.
-
-
-    rewrite !map_length.
 
 (*The main part: prove related*)
 Theorem elim_let_related (tsk1 : TaskDefs.task) (tsk2 : Task.task):
@@ -888,7 +1569,29 @@ Proof.
   (*Now decompose bind again: first just gives us [elim_let_f goal], second
     builds the task*)
   (*TODO: think we will need to prove that result of [elim_let_f] is alpha equivalent*)
-  eapply prove_errst_spec_bnd with (Q1:=fun _ f2 _ => eval_fmla f2 = Some (elim_let_f true true goal))
+  (*NOTE: don't think we can say eval_fmla =, need fmla_related*)
+  Check fmla_related.
+  eapply prove_errst_spec_bnd with (Q1:=fun _ f2 _ => fmla_related f2 (elim_let_f true true goal))
+  (Q2:=fun x _ y _ => task_related (Some y) (gamma1, delta1, elim_let_f true true goal1))
+  (P2:=fun x _ => fmla_related x (elim_let_f true true goal)) (*TODO: see*); auto.
+  2: { (*Prove ending spec assuming [elim_let] correct*) intros f2. apply prove_errst_spec_ret. intros _ Hf2.
+    unfold task_related.
+    exists (gamma, delta, (elim_let_f true true goal)).
+    split.
+    - unfold eval_task. simpl.
+      (*TODO: prove these equal in separate lemmas for [change_*] lemmas since we change goal *)
+      admit.
+    - unfold a_equiv_task. simpl_task. bool_to_prop; split_all; auto.
+      (*Why we needed that a_equiv_f is preserved by elim_let_f*)
+      apply elim_let_f_a_equiv; auto.
+  }
+  (*TODO: prove that these transformations related. NOTE: everything up to now wasnt super
+    specific to [elim_let] and it could/should be refactored*)
+  (*TODO: weaken precondition and use separate lemma*)
+Admitted.
+(* 
+
+eapply prove_errst_spec_bnd with (Q1:=fun _ f2 _ => eval_fmla f2 = Some (elim_let_f true true goal))
   (Q2:=fun x _ y _ => task_related (Some y) (gamma1, delta1, elim_let_f true true goal1))
   (P2:=fun x _ => eval_fmla x = Some (elim_let_f true true goal)) (*TODO: see*); auto.
   2: { (*Prove ending spec assuming [elim_let] correct*) intros f2. apply prove_errst_spec_ret. intros _ Hf2.
@@ -908,8 +1611,7 @@ Proof.
   }
   (*TODO: prove that these transformations related. NOTE: everything up to now wasnt super
     specific to [elim_let] and it could/should be refactored*)
-  (*TODO: weaken precondition and use separate lemma*)
-Admitted.
+  (*TODO: weaken precondition and use separate lemma*) *)
 
 
 Theorem elim_let_sound: trans_errst_sound elim_let.
